isabelle/DeBruijnVar.thy
@@ -1,0 +1,79 @@
+theory DeBruijnVar
+imports Main
+begin
+
+datatype var = DBVar nat
+
+definition first :: var
+where "first = DBVar 0"
+
+primrec "next" :: "var => var"
+where "next (DBVar v) = DBVar (Suc v)"
+
+primrec next_by :: "nat => var => var"
+where "next_by n (DBVar v) = DBVar (v + n)"
+
+fun incr :: "var => var => var"
+where "incr (DBVar n) (DBVar v) = DBVar (if v < n then v else Suc v)" 
+
+fun subr :: "var => var => var"
+where "subr (DBVar n) (DBVar v) = DBVar (if v > n then v - 1 else v)" 
+
+fun canswap :: "var => var => bool"
+where "canswap (DBVar m) (DBVar n) = (m <= n)" 
+
+lemma [simp]: "subr n (incr n var) = var"
+by (induction n, induction var, simp)
+
+lemma [simp]: "incr n n = next n"
+by (induction n, simp)
+
+lemma [simp]: "next v ~= v"
+by (induction v, simp)
+
+lemma [simp]: "subr v (next v) = v"
+by (induction v, simp)
+
+lemma [simp]: "incr v x ~= v"
+by (induction v, induction x, simp)
+
+lemma [simp]: "next_by 0 v = v"
+by (induction v, simp)
+
+lemma [simp]: "next_by x (next v) = next (next_by x v)"
+by (induction v, simp)
+
+lemma [simp]: "next_by (Suc x) v = next (next_by x v)"
+by (induction v, simp)
+
+lemma [simp]: "canswap m n ==> incr m (incr n var) = incr (next n) (incr m var)"
+by (induction var, induction n, induction m, simp)
+
+lemma [simp]: "canswap first x"
+by (induction x, simp add: first_def)
+
+lemma [simp]: "canswap m n ==> canswap m (next n)"
+by (induction n, induction m, simp)
+
+lemma [simp]: "canswap m n ==> canswap (next m) (next n)"
+by (induction n, induction m, simp)
+
+lemma [simp]: "canswap m n ==> canswap (next_by x m) (next_by x n)"
+by (induction n, induction m, simp)
+
+lemma [simp]: "canswap var del ==> canswap (incr n var) (next del)"
+by (induction del, induction n, induction var, simp)
+
+lemma [simp]: "canswap n del ==> canswap v (next del) ==> canswap (subr n v) del"
+by (induction del, induction n, induction v, auto)
+
+lemma [simp]: "canswap m n ==> incr m (subr n v) = subr (next n) (incr m v)"
+by (induction m, induction n, induction v, auto)
+
+lemma [simp]: "canswap m n ==> incr m n = next n"
+by (induction m, induction n, simp)
+
+lemma [simp]: "canswap m n ==> v ~= n ==> incr m v ~= next n"
+by (induction m, induction n, induction v, simp)
+
+end
